# Problem 1

Find $(AB)^{T}$

$$
A = \begin{pmatrix}
1^{2} & 2^{2} & 3^{2}  & \dots &  n^{2} \\
2 ^{2}  & & \dots & & (n+1)^{2} \\
. \\
. \\
m^{2} &  & \dots & & (m + n - 1) ^{2}
\end{pmatrix}
$$

$$
B = \begin{pmatrix}
1^{2} & 2^{2} & 3^{2}  & \dots &  p^{2} \\
2 ^{2}  & & \dots & & (n+1)^{2} \\
. \\
. \\
n^{2} &  & \dots & & (n + p - 1) ^{2}
\end{pmatrix}
$$

## Solution

$$
\begin{align}
(B^{T} A ^{T})_{3,4} &= 3^{2} \cdot 4 + 4 ^{2} \cdot 5 \dots (n + 2)^{2} \cdot (n+3) \\
&= \sum_{i=3}^{n + 2} i(i + 1)^{2} \\
&= \sum_{i=3}^{n + 2} i^{3} + 2i^{2} + i \\
&=  \frac{((n + 2)(n + 3))^{2}}{4} - \frac{(2\cdot{3})^{2}}{4} + 2\left(\frac{(n + 2)(n + 3)(2n + 5)}{6} - \frac{(2)(3)(5)}{6}\right) + \frac{(n + 2)(n + 3)}{2} - \frac{2(3)}{2}\\
&= \frac{(n + 2)(n + 3)}{2} - 22
\end{align}
$$

# Problem 2

Find $(\mathbf{A}\mathbf{B})^{T}$

$$
\begin{align}
A &= \begin{pmatrix}
1 & \dots & \frac{1}{n} \\
\frac{1}{2} & \dots & \frac{1}{n + 1}\\
\dots
\end{pmatrix}
B &= \begin{pmatrix}
\frac{1}{2} & \dots & \frac{1}{p + 1} \\
\frac{1}{3} & \dots & \frac{1}{n + 2}\\
\dots
\end{pmatrix}
\end{align}
$$

## Solution

$$
\begin{align}
(\mathbf{A}\mathbf{B})^{T} &= \sum_{i=3}^{n + 2} \frac{1}{i(i + 1)} \\
&= \sum_{i=3}^{n + 2} \frac{1}{i} - \frac{1}{i + 1} \\ \\
&= \frac{1}{3} - \frac{1}{n + 3} \\
&= \frac{n}{n + 3}
\end{align}
$$

