# Discrete

## p 371 6

$$
\begin{align}
a_{0} &= 4 \\
a_{1} &= 13 \\
a_{n} &= 3a_{n-1} + 10a_{n-2}
\end{align}
$$

We assume the form

$$
a_{n} = r^{n}
$$

From there,

$$
\begin{align}
r^{n} &= 3r^{n - 1} + 10r^{n - 2} \\
r^{n} - 3r^{n-1} - 10r^{n-2} &= 0 \\
r^{n-2}(r^{2} - 3r - 10) &= 0 \\
r^{n-2}(r + 2)(r - 5) &= 0 \\
r = -2, 5
\end{align}
$$

So

$$
\begin{align}
a_{n} &= R(-2)^{n} + S(5)^{n} \\
\end{align}
$$
$$
\begin{cases}
a_{0} = 4 = R + S \\
a_{1} = 13 = -2R + 5S
\end{cases}
$$

and we get

$$
R = 1, S = 3
$$

The general form for $a_{n}$ is

$$
a_{n} = (-2)^{n} + 3(5)^{n}
$$