# Example 1

$$
\begin{equation}
\begin{cases}
x_{1} + x_{2} - x_{3} = 0 \\
x_{1} - 4x_{2} + 3x_{3} = 0 \\
-5x_{1} + 13x_{2} -10 x_{3} = 0
\end{cases}
\end{equation}
$$

Augmented Matrix:

$$
\begin{pmatrix}
1 & 1 & -1 & 0 \\
2 & -4 & 3 & 0 \\
-5 & 13 & -10 & 0
\end{pmatrix} 
$$

Solving:

$$
\begin{align}
R_{2} - 2R_{1}, R_{3} + 5R_{1} &\implies \begin{pmatrix}
1 & 1 & -1 & 0 \\
0 & -6 & 5 & 0 \\
0 & 0 & 0 & 0
\end{pmatrix} \\
x_{3} = t &\implies x_{2} = \frac{5}{6}t, x_{1} = \frac{1}{6}t
\end{align}
$$

# Example 2

$$
\begin{equation}
\begin{cases}
x_{1} - 2x_{2} + x_{3} + x_{4} = 2 \\
3x_{1} + 2x_{3} - 2x_{4} = 0 \\
4x_{2} - x_{3} + x_{4} = 9 \\
-x_{1} + 6x_{2} - 2x_{3} = 7
\end{cases}
\end{equation}
$$

Augmented Matrix:

$$
\begin{pmatrix}
1 & -2 & 1 & 1 & 2 \\
3 & 0 & 2 & -2 & 0 \\
0 & 4 & -1 & 1 & 9 \\
-1 & 6 & -2 & 0 & 7
\end{pmatrix}
$$

Solution:

$$
\begin{align}
R_{2} \to R_{2} - 3R_{1}, R_{4} \to R_{4} + R_{1} - R_{3} &\implies \begin{pmatrix}
1 & -2 & 1 & 1 & 2\\
0 & 6 & -1 & -5 & -6 \\
0 & 4 & -1 & 1 & 9 \\
0 & 0 & 0 & 0 & 0
\end{pmatrix} \\
R_{3} \to R_{3} - \frac{2}{3}R_{2}, \, R_{2} \to \frac{1}{6}R_{2} &\implies \begin{pmatrix}
1 & -2 & 1 & 1 & 2 \\
0 & 1 & -\frac{1}{6} & -\frac{5}{6} & -1 \\
0 & 0 & -\frac{1}{3} & \frac{13}{3} & 13 \\
0 & 0 & 0 & 0 & 0 \\
\end{pmatrix} \\
\end{align}
$$

$$
x_{4} = t \implies 
\begin{equation}
\begin{cases}
-\frac{1}{3}x_{3} - \frac{13}{3}t = 13 \implies x_{3} = -39 + 13t \\
x_{2} + \frac{13}{2} - \frac{13}{6}t - \frac{5}{6}t = -1 \implies x_{2} = -\frac{13}{2} + 3t \\
x_{1} + 13 - 6t -39 + 13t + t = 2 \implies x_{1} = 28 - 8t
\end{cases}
\end{equation}
$$

$$
\vec{x} = t\begin{pmatrix}
-8 \\
3 \\
13 \\
1
\end{pmatrix} + \begin{pmatrix}
28 \\
-\frac{13}{2} \\
-39 \\
1
\end{pmatrix}
$$