# Problem 1

Prove 

$$
\sum_{i=1}^{n} i^{3} = \frac{n^{2}(n+1)^{2}}{4}
$$

## Solution

Base case:

$$
S(1) = 1^{3} = 1
$$

The base case is true. Now we prove the induction:

$$
\begin{align}
S(n) + (n + 1)^{3} &= \frac{n^{2}(n + 1)^{2}}{4} + (n + 1)^{3} \\
&= \frac{(n^{2}+4(n + 1))(n + 1)^{2}}{4} \\
&= \frac{(n + 1)^{2}(n + 2)^{2}}{4} \\
&= S(n + 1)
\end{align}
$$
Proven.

# Problem 2

Find the inverse of 

$$
\mathbf{A} = \begin{pmatrix}
1 &  & \dots &  &  \\
& \frac{1}{2} & \dots &  &  \\
& & \frac{1}{3} &  &  \\
& &  & \frac{1}{n}
\end{pmatrix}
$$

## Solution


$$
\mathbf{C} = \begin{pmatrix}
1 & \dots & \dots & \dots  \\
\dots& 2 & \dots &  \dots  \\
\dots& \dots & 3 &  \dots  \\
\dots&\dots &\dots & n
\end{pmatrix}
$$

# Problem 3

## Part 1

Prove if $\mathbf{A}$ is invertible, then $(\mathbf{A}^{-1})^{-1} = \mathbf{A}$

## Solution

Definition of inverse states that the relationship holds true both ways.

## Part 2

Prove

$$
\begin{align}
(AB)^{-1} &= B^{-1}A^{-1} \\
\implies AB \cdot(B^{-1}A^{-1}) &= I \\
\end{align}
$$

## Solution

$$
\begin{align}
AB(B^{-1}A^{-1}) &= (AB(B^{-1}))A^{-1} \\
&= (AI)A^{-1} \\
&= I
\end{align}
$$

## Part 3

Prove 

$$
(BA)^{-1} = A^{-1}B^{-1}
$$

## Solution

$$
\begin{align}
(BA)(A^{-1}B^{-1}) &= (BA A^{-1})(B^{-1}) \\
&= (BI)(B^{-1}) \\
&= B B^{-1} \\
&= I
\end{align}
$$

