# Quiz 7

a. $$
\begin{bmatrix}
-2 & 3 & 1 
\end{bmatrix} \cdot
\begin{bmatrix}
-1 \\
4  \\
 2
\end{bmatrix} = -2 \cdot -1 + 3 \cdot 4 + 1 \cdot 2 =16
$$

b. $$
\begin{align}
\begin{bmatrix}
3 & -2 & 1 & 4 & 3 & 6 & 8
\end{bmatrix} \cdot \begin{bmatrix}
-2 \\
-2 \\
4 \\
-6 \\
3 \\
1 \\
0
\end{bmatrix} &= 3 \cdot -2 + -2 \cdot -2 + 1 \cdot 4 + 4 \cdot -6 + 3 \cdot 3 + 6 \cdot 1 + 8 \cdot 0 \\
&= -7

\end{align}
$$
# Problem 1

Theorem states that $A_{n\times n}, B_{n\times n}$ are invertible $\implies (AB)^{-1} = B^{-1} \cdot A^{-1}$

Prove that $A_{1}, A_{2}, A_{3} \dots A_{n}$ are invertible matrices. Or equivalently,

$$
(A_{1} \cdot A_{2} \cdot A_{3} \dots A_{n}) ^{-1} = A_{n}^{-1} \cdot A_{n - 1}^{-1} \dots A_{1}^{-1}
$$

Base case: n = 2

The theorem literally states this is true

Inductive step: 

Let $A = (A_{1} \cdot A_{2} \dots A_{n})$, $B = A_{n + 1}$

$$
\begin{align}
(A_{1} \cdot A_{2} \dots A_{n+1})^{-1} &= (A \cdot B)^{-1} \\
&= B^{-1} \cdot A^{-1} \\
&= A_{n + 1}^{-1} \cdot A_{n}^{-1} \cdot A_{n - 1}^{-1} \dots A_{1}
\end{align}
$$

$S(n+ 1)$ holds true given $S(n)$ is true.