$$
\begin{align}
R_{2} \leftrightarrow  R_{3} &= \begin{bmatrix}
-6 & 0 & 4 \\
3 & 5 & 8 \\
2 & -4 & 8
\end{bmatrix} \\
R_{1} \to -\frac{1}{6}R_{1} &= \begin{bmatrix}
1 & 0 & -\frac{2}{3}\\
3 & 5 & 8 \\
2 & -4 & 8
\end{bmatrix}\\ 
R_{2} \to R_{2} - 3R_{1} &= \begin{bmatrix}
1 & 0 & -\frac{2}{3}\\
0 & 5 & 10 \\
2 & -4 & 8
\end{bmatrix} \\
R_{2} \to \frac{1}{5}R_{2} &= \begin{bmatrix}
1 & 0 & -\frac{2}{3}\\
0 & 1 & 2 \\
2 & -4 & 8
\end{bmatrix} \\
R_{3} \to \frac{3}{52}( R_{3} - 2R_{1} + 4R_{2}) &=\begin{bmatrix}
1 & 0 & -\frac{2}{3}\\
0 & 1 & 2 \\
0 & 0 & 1
\end{bmatrix}
\end{align}
$$